theories/paper.v
@@ -8,16 +8,16 @@ From det Require Import t2l valid_tree elpi elpi_equiv.
 
 (*prooftree: runbp*)
 (*SNIP: run_sig *)
-Inductive run (u:Unif) (p : program): fvS -> Sigma -> tree -> 
+Inductive runT (u:Unif) (p : program): fvS -> Sigma -> tree -> 
                   Sigma -> option tree -> Prop :=
 (*ENDSNIP: run_sig *)
-  | run_done s1 s2 A B fv            : success A -> get_subst s1 A = s2 -> (next_alt true A) = B -> run fv s1 A s2 B
-  | run_step  s1 s2 r A B fv0 fv1 st : path_atom A -> step u p fv0 s1 A = (fv1, st, B) -> run fv1 s1 B s2 r -> run fv0 s1 A s2 r
-  | run_fail s1 s2 A B r fv0         : failed A -> next_alt false A = Some B -> run fv0 s1 B s2 r -> run fv0 s1 A s2 r.
+  | run_done s1 s2 A B fv            : success A -> get_subst s1 A = s2 -> (next_alt true A) = B -> runT fv s1 A s2 B
+  | run_step  s1 s2 r A B fv0 fv1 st : path_atom A -> step u p fv0 s1 A = (fv1, st, B) -> runT fv1 s1 B s2 r -> runT fv0 s1 A s2 r
+  | run_fail s1 s2 A B r fv0         : failed A -> next_alt false A = Some B -> runT fv0 s1 B s2 r -> runT fv0 s1 A s2 r.
 (*endprooftree: runbp*)
 
 Lemma run_runT u p fv s0 t0 s1 t1:
-  run u p fv s0 t0 s1 t1 -> (exists b fv1, tree.run u p fv s0 t0 (Some s1) t1 b fv1).
+  runT u p fv s0 t0 s1 t1 -> (exists b fv1, tree.run u p fv s0 t0 (Some s1) t1 b fv1).
 Proof.
   elim => >.
   - move=> sA <-<-; repeat eexists.
@@ -30,7 +30,7 @@ Qed.
 
 
 Lemma runT_run u p fv s0 t0 sx t1 b fv1:
-  tree.run u p fv s0 t0 (Some sx) t1 b fv1 -> run u p fv s0 t0 sx t1.
+  tree.run u p fv s0 t0 (Some sx) t1 b fv1 -> runT u p fv s0 t0 sx t1.
 Proof.
   remember (Some sx) as ss eqn:Hss.
   move=> H; elim_run H sx Hss.
@@ -52,7 +52,7 @@ Open Scope my_scope.
 Lemma tree_to_elpi: forall u p s0 t s2 t',
   let fv := vars_tree t `|` vars_sigma s0 in
   valid_tree t ->
-    run u p fv s0 t s2 t' -> 
+    runT u p fv s0 t s2 t' -> 
       exists s1 g a,
         let: na := (t2l (odflt KO t') s0 [::]) in
         t2l t s0 [::] = (s1,g) :: a /\
@@ -69,7 +69,7 @@ Qed.
 Lemma elpi_to_tree: forall u p fv s1 g s2 a na,
   nur u p fv s1 g a s2 na -> 
     forall s0 t, valid_tree t -> t2l t s0 [::] = (s1,g) :: a -> 
-      exists t', run u p fv s0 t s2 t' /\ t2l (odflt KO t') s0 [::] = na.
+      exists t', runT u p fv s0 t s2 t' /\ t2l (odflt KO t') s0 [::] = na.
 (*ENDSNIP: elpi_to_tree *)
 Proof.
   move=> > H1 H2 H3 H4 H5.
